src/simulation/FtoCoherent.v
@@ -1,0 +1,212 @@
+Require Import PArith Setoid.
+From hahn Require Import Hahn.
+Require Import PromisingLib.
+Require Import FLocHelper.
+From Promising2 Require Import TView View Time Event Cell Thread Memory Configuration Local.
+
+From imm Require Import Events Execution.
+From imm Require Import imm_s_hb.
+From imm Require Import imm_s.
+From imm Require Import CombRelations.
+From imm Require Import TraversalConfig.
+From imm Require Import ProgToExecution.
+From imm Require Import ProgToExecutionProperties.
+
+Set Implicit Arguments.
+Remove Hints plus_n_O.
+
+Section FtoCoherent.
+Variable G : execution.
+Variable WF : Wf G.
+Variable sc : relation actid.
+Variable IMMCON : imm_consistent G sc.
+Variable I : actid -> Prop.
+
+Notation "'acts'" := G.(acts).
+Notation "'co'" := G.(co).
+Notation "'coi'" := G.(coi).
+Notation "'sw'" := G.(sw).
+Notation "'sb'" := G.(sb).
+Notation "'rf'" := G.(rf).
+Notation "'rfe'" := G.(rfe).
+Notation "'rmw'" := G.(rmw).
+Notation "'lab'" := G.(lab).
+Notation "'msg_rel'" := (msg_rel G sc).
+Notation "'urr'" := (urr G sc).
+
+Notation "'E'" := G.(acts_set).
+Notation "'R'" := (fun a => is_true (is_r lab a)).
+Notation "'W'" := (fun a => is_true (is_w lab a)).
+Notation "'F'" := (fun a => is_true (is_f lab a)).
+Notation "'Loc_' l" := (fun x => loc lab x = Some l) (at level 1). (* , format "'Loc_'  l"). *)
+Notation "'Tid_' t" := (fun x => tid x = t) (at level 1).
+Notation "'W_'" := (fun l => W ∩₁ Loc_ l).
+(* Notation "'RW'" := (fun x => R x \/ W x). *)
+Notation "'FR'" := (fun x => F x \/ R x).
+Notation "'FW'" := (fun x => F x \/ W x).
+
+Notation "'Pln'" := (fun a => is_true (is_only_pln lab a)).
+Notation "'Rlx'" := (is_rlx lab).
+Notation "'Rel'" := (is_rel lab).
+Notation "'Acq'" := (is_acq lab).
+Notation "'Acqrel'" := (is_acqrel lab).
+Notation "'Sc'" := (fun a => is_true (is_sc lab a)).
+
+Notation "'W_ex'" := G.(W_ex).
+Notation "'W_ex_acq'" := (W_ex ∩₁ (fun a => is_true (is_xacq lab a))).
+  
+Variable IE : I ⊆₁ E ∩₁ W.
+Variable INITINI: is_init ∩₁ E ⊆₁ I.
+Variables f_to f_from : actid -> Time.t.
+
+Definition f_to_coherent :=
+  (* ⟪ NW  : forall a, ~ is_w lab a -> f_to a = tid_init ⟫ /\ *)
+  ⟪ TINITTO : forall x, (is_init ∩₁ E) x -> f_to x = tid_init ⟫ /\
+  ⟪ TINITFROM : forall x, (is_init ∩₁ E) x -> f_from x = tid_init ⟫ /\
+  ⟪ TTOFROM : forall x,
+      I x -> ~ is_init x -> Time.lt (f_from x) (f_to x) ⟫ /\
+  ⟪ TCO : forall x y,
+      I x -> I y ->
+      co x y -> Time.le (f_to x) (f_from y) ⟫ /\
+  ⟪ TRMW : forall x y,
+      I x -> I y -> (rf ⨾ rmw) x y -> f_to x = f_from y ⟫
+.
+
+Section Props.
+
+Variable FCOH : f_to_coherent.
+
+Lemma f_to_co_mon e e' (CO : co e e') (ISS : I e) (ISS' : I e') :
+  Time.lt (f_to e) (f_to e').
+Proof.
+  eapply TimeFacts.le_lt_lt.
+  2: eapply FCOH; auto.
+  { by apply FCOH. }
+  apply Execution_eco.no_co_to_init in CO; auto.
+  { apply seq_eqv_r in CO. desf. }
+  apply coherence_sc_per_loc.
+  apply IMMCON.
+Qed.
+
+Lemma f_from_co_mon e e' (NINIT : ~ is_init e) (CO : co e e') (ISS : I e) (ISS' : I e') :
+  Time.lt (f_from e) (f_from e').
+Proof.
+  eapply TimeFacts.lt_le_lt.
+  { eapply FCOH; eauto. }
+    by apply FCOH.
+Qed.
+
+Lemma f_to_coherent_strict x y z (ISSX : I x) (ISSY : I y) (ISSZ : I z)
+      (COXY: co x y) (COYZ: co y z) :
+  Time.lt (f_to x) (f_from z).
+Proof.
+  eapply TimeFacts.le_lt_lt.
+  { apply FCOH.
+    3: by apply COXY.
+    all: eauto. }
+  eapply f_from_co_mon; eauto.
+  apply Execution_eco.no_co_to_init in COXY; auto.
+  { apply seq_eqv_r in COXY. desf. }
+  apply coherence_sc_per_loc.
+  apply IMMCON.
+Qed.
+
+Lemma lt_init_ts e (EE : E e) (WW : W e) (ISS : I e) (NINIT : ~ is_init e) :
+  Time.lt tid_init (f_to e).
+Proof.
+  unfold is_w in *.
+  destruct e; desf.
+  cdes FCOH.
+  assert (E (InitEvent l)) as EL.
+  { apply WF.(wf_init). eexists.
+    split; eauto. unfold loc. desf. }
+  assert ((is_init ∩₁ E) (InitEvent l)) as LL.
+  { by split; eauto. }
+  erewrite <- TINITTO; eauto.
+  eapply f_to_co_mon; eauto.
+  eapply init_co_w; eauto.
+  { unfold is_w. desf. }
+  red. unfold loc. rewrite WF.(wf_init_lab).
+  desf.
+Qed.
+
+Lemma le_init_ts e (EE : E e) (WW : W e) (ISS : I e) :
+  Time.le tid_init (f_to e).
+Proof.
+  unfold is_w in *.
+  destruct e; desf.
+  { apply Time.le_lteq. right.
+    symmetry. cdes FCOH. apply TINITTO.
+    split; auto. }
+  apply Time.le_lteq. left.
+  eapply lt_init_ts; eauto.
+  unfold is_w. desf.
+Qed.
+
+Lemma le_init_ts_from e (EE : E e) (WW : W e) (ISS : I e) (NINIT : ~ is_init e) :
+  Time.le tid_init (f_from e).
+Proof.
+  unfold is_w in *.
+  destruct e; desf.
+  cdes FCOH.
+  assert (E (InitEvent l)) as EL.
+  { apply WF.(wf_init). eexists.
+    split; eauto. unfold loc. desf. }
+  assert ((is_init ∩₁ E) (InitEvent l)) as LL.
+  { by split; eauto. }
+  erewrite <- TINITTO; eauto.
+  apply FCOH; eauto.
+  eapply init_co_w; eauto.
+  { unfold is_w. desf. }
+  red. unfold loc. rewrite WF.(wf_init_lab).
+  desf.
+Qed.
+
+Lemma f_to_eq e e' (SAME_LOC : same_loc lab e e') (ISS : I e) (ISS' : I e')
+      (FEQ : f_to e = f_to e') :
+  e = e'.
+Proof.
+  assert (E e /\ E e') as [EE EE']. 
+  { by split; apply IE. }
+  assert (W e /\ W e') as [WE WE']. 
+  { by split; apply IE. }
+  destruct (classic (e = e')) as [|NEQ]; auto.
+  exfalso.
+  edestruct (wf_co_total WF); eauto.
+  1,2: split; [split|]; eauto.
+  { assert (Time.lt (f_to e) (f_to e')) as HH.
+    { eapply f_to_co_mon; eauto. }
+    rewrite FEQ in *.
+      by apply DenseOrder.lt_strorder in HH. }
+  assert (Time.lt (f_to e') (f_to e)) as HH.
+  { eapply f_to_co_mon; eauto. }
+  rewrite FEQ in *.
+    by apply DenseOrder.lt_strorder in HH.
+Qed.
+
+Lemma f_from_eq e e' (SAME_LOC : same_loc lab e e') (ISS : I e) (ISS' : I e')
+      (NINIT : ~ is_init e) (NINIT' : ~ is_init e')
+      (FEQ : f_from e = f_from e') :
+  e = e'.
+Proof.
+  assert (E e /\ E e') as [EE EE']. 
+  { by split; apply IE. }
+  assert (W e /\ W e') as [WE WE']. 
+  { by split; apply IE. }
+  destruct (classic (e = e')) as [|NEQ]; auto.
+  exfalso.
+  edestruct (wf_co_total WF); eauto.
+  1,2: split; [split|]; eauto.
+  { assert (Time.lt (f_from e) (f_from e')) as HH.
+    { eapply f_from_co_mon; eauto. }
+    rewrite FEQ in *.
+      by apply DenseOrder.lt_strorder in HH. }
+  assert (Time.lt (f_from e') (f_from e)) as HH.
+  { eapply f_from_co_mon; eauto. }
+  rewrite FEQ in *.
+    by apply DenseOrder.lt_strorder in HH.
+Qed.
+
+End Props.
+
+End FtoCoherent.
